example/ttl: Finish derivation without admits

src/Rupicola/Examples/Ttl/Ttl.v
@@ -1,8 +1,5 @@
 Require Import Rupicola.Lib.Api.
-
-(* Definition packet := *)
-(*   hlist.t ["field1"; …; "ttl"] [Byte.byte; …; Byte.byte]. (* field1, ttl *) *)
-(* FIXME move to VectorArray.t *)
+Require Import Rupicola.Lib.Arrays.
 
 Section with_parameters.
   Context {width: Z} {BW: Bitwidth width} {word: word.word width} {mem: map.map word Byte.byte}.
@@ -14,180 +11,44 @@ Section with_parameters.
   Context {env_ok : map.ok env}.
   Context {ext_spec_ok : Semantics.ext_spec.ok ext_spec}.
 
-  Context {width_sufficient : (2 < 2 ^ width)%Z}. (* without this, we have no guarantee that index 2 fits in the allowed integer size *)
-
   Definition packet :=
     Vector.t word 2. (* field1, ttl *)
 
-  Notation field1_index := Fin.F1.
-  Notation ttl_index := (Fin.FS Fin.F1).
-  Notation field1 p := (Vector.nth p field1_index).
-  Notation ttl p := (Vector.nth p ttl_index).
+  Definition __lt {a b: nat} : if lt_dec a b return Prop then a < b else True :=
+    match lt_dec a b as c return (if c return Prop then a < b else True) with
+    | left pr => pr
+    | _ => I
+    end.
 
-  Definition WordVector {n} (addr: word) (v: Vector.t word n) : mem -> Prop :=
-    array scalar (word.of_Z 8) addr (Vector.to_list v).
+  Notation _lt :=
+    ltac:(lazymatch goal with
+          | [  |- ?a < ?b ] => exact (@__lt a b)
+          end) (only parsing).
 
-  Definition Packet (addr: word) (p: packet)
-    : mem -> Prop :=
-    WordVector addr p.
+  Notation ttl_idx := 1.
+  Definition field1 (p: packet) := (VectorArray.get p 0 _lt).
+  Definition ttl (p: packet) := (VectorArray.get p ttl_idx _lt).
+
+  Definition Packet (addr: word) (p: packet) : mem -> Prop :=
+    vectorarray_value AccessWord addr p.
 
   Definition decr_gallina (p: packet) :=
     let/n ttl := (ttl p) in
-    let/n m1 := word.of_Z (-1) in
-    let/n ttl := word.add ttl m1 in
-    let/n p := Vector.replace p ttl_index ttl in
+    let/n ttl := word.add ttl (word.of_Z (-1)) in
+    let/n p := VectorArray.put p ttl_idx _lt ttl in
     p.
-
-  Lemma vector_uncons {A n} (v: Vector.t A n) :
-    match n return Vector.t A n -> Prop with
-    | 0 => fun v => v = Vector.nil _
-    | S n =>fun v => v = Vector.cons _ (Vector.hd v) _ (Vector.tl v)
-    end v.
-  Proof.
-    destruct v; reflexivity.
-  Qed.
-
-  Lemma Vector_to_list_length {A n} (v: Vector.t A n):
-    Datatypes.length (Vector.to_list v) = n.
-  Proof. Admitted.
-
-  Lemma compile_nth : forall {n} {tr mem locals functions}
-        (vector: Vector.t word n) offset,
-    let v := Vector.nth vector offset in
-    let noffset := proj1_sig (Fin.to_nat offset) in
-    forall {P} {pred: P v -> predicate} {k: nlet_eq_k P v} {k_impl}
-      R vector_ptr vector_var var,
-
-      (Z.of_nat n < 2 ^ width)%Z ->
-
-      sep (WordVector vector_ptr vector) R mem ->
-      map.get locals vector_var = Some vector_ptr ->
-
-      (let v := v in
-       forall m,
-         sep (WordVector vector_ptr vector) R m ->
-         <{ Trace := tr;
-            Memory := m;
-            Locals := map.put locals var v;
-            Functions := functions }>
-         k_impl
-         <{ pred (k v eq_refl) }>) ->
-      <{ Trace := tr;
-         Memory := mem;
-         Locals := locals;
-         Functions := functions }>
-      (cmd.seq (cmd.set
-                  var
-                  (expr.load
-                     access_size.word
-                     (expr.op bopname.add
-                              (expr.var vector_var)
-                              (expr.literal ((@word.unsigned _ word (word.of_Z 8) * Z.of_nat noffset))))))
-               k_impl)
-      <{ pred (nlet_eq [var] v k) }>.
-  Proof.
-    intros.
-    unfold WordVector in *.
-    repeat straightline.
-    exists (word.of_Z (word.unsigned v)).
-    split.
-    { repeat straightline; eauto.
-      exists vector_ptr; intuition.
-      seprewrite_in @array_index_nat_inbounds H0;
-        cycle 1.
-      { eexists.
-        split.
-        { eapply load_word_of_sep.
-          ecancel_assumption. }
-      { subst v.
-        (* FIXME: vector/list lemmas *)
-        admit. } }
-      { rewrite Vector_to_list_length.
-        apply (proj2_sig (Fin.to_nat offset)). } }
-    { repeat straightline.
-      cbv [dlet.dlet].
-      subst l.
-      rewrite word.of_Z_unsigned.
-      eauto. }
-    Unshelve.
-    apply (word.of_Z 0).
-  Admitted.
-
-  Lemma compile_replace : forall {n} {tr mem locals functions}
-        (vector: Vector.t word n) offset value,
-    let v := (Vector.replace vector offset value) in
-    let noffset := proj1_sig (Fin.to_nat offset) in
-    forall {P} {pred: P v -> predicate} {k: nlet_eq_k P v} {k_impl}
-      R vector_ptr vector_var value_var,
-
-      (Z.of_nat n < 2 ^ width)%Z ->
-      sep (WordVector vector_ptr vector) R mem ->
-
-      map.get locals vector_var = Some vector_ptr ->
-      map.get locals value_var = Some value ->
-
-      (let v := v in
-       forall m,
-         sep (WordVector vector_ptr v) R m ->
-         <{ Trace := tr;
-            Memory := m;
-            Locals := locals;
-            Functions := functions }>
-         k_impl
-         <{ pred (k v eq_refl) }>) ->
-      <{ Trace := tr;
-         Memory := mem;
-         Locals := locals;
-         Functions := functions }>
-      cmd.seq (cmd.store access_size.word
-                         (expr.op bopname.add
-                                  (expr.var vector_var)
-                                  (expr.literal ((@word.unsigned _ word (word.of_Z 8) *
-                                                  Z.of_nat noffset))))
-                         (expr.var value_var))
-              k_impl
-      <{ pred (nlet_eq [vector_var] v k) }>.
-  Proof.
-    intros.
-    unfold WordVector in *.
-    repeat straightline.
-    exists (word.add vector_ptr
-                     (word.of_Z (@word.unsigned _ word (word.of_Z 8) * Z.of_nat noffset))).
-    split.
-    { repeat straightline; eauto.
-      exists vector_ptr; intuition.
-      reflexivity. }
-    { exists value.
-      split.
-      { straightline.
-        eexists; eauto. }
-      { repeat straightline.
-        eapply store_word_of_sep.
-        { seprewrite_in @array_index_nat_inbounds H0;
-            cycle 1.
-          { ecancel_assumption. }
-          { subst noffset.
-            rewrite Vector_to_list_length.
-            apply (proj2_sig (Fin.to_nat offset)). } }
-        { intros.
-          apply H3.
-          seprewrite (array_index_nat_inbounds (default:=word.of_Z 0) scalar (word.of_Z 8) (Vector.to_list v) vector_ptr (proj1_sig (Fin.to_nat offset))); cycle 1.
-          { admit.                (* Lemmas on Vector.to_list and replace *)
-          }
-          { subst noffset.
-            rewrite Vector_to_list_length.
-            apply (proj2_sig (Fin.to_nat offset)). } }
-  Admitted.
 
   Hint Unfold Packet : compiler_cleanup.
 
   Instance spec_of_decr : spec_of "decr" :=
     fnspec! "decr" ptr / p R,
-    { requires tr mem := (Packet ptr p ⋆ R) mem;
-      ensures tr' mem' := tr' = tr /\ (Packet ptr (decr_gallina p) ⋆ R) mem' }.
+    { requires tr mem :=
+        (Packet ptr p ⋆ R) mem;
+      ensures tr' mem' :=
+        tr' = tr /\ (Packet ptr (decr_gallina p) ⋆ R) mem' }.
 
-  Hint Extern 1 => simple eapply compile_nth; shelve : compiler.
-  Hint Extern 1 => simple eapply compile_replace; shelve : compiler.
+  Import VectorArrayCompiler.
+  Hint Unfold ttl : compiler_cleanup.
 
   Derive decr_body SuchThat
          (defn! "decr"("p") { decr_body },
